immutable-btree/BtreeImpl.dfy
@@ -2,88 +2,86 @@ include "../lib/total_order.dfy"
 include "../lib/map_utils.dfy"
 include "../lib/mathematics.dfy"
 include "../lib/sequences.dfy"
-include "BtreeSpec.dfy"
 include "BtreeInv.dfy"
 
 abstract module BtreeImpl {
-  import opened BtreeSpec
-  import opened BtreeInv
+  import opened Inv : BtreeInv
   import opened Sequences
 
-  lemma strictlySortedInsert(l: seq<Key>, k: Key, pos: int)
+  lemma strictlySortedInsert(l: seq<Spec.Key>, k: Spec.Key, pos: int)
   requires -1 <= pos < |l|;
-  requires Keyspace.IsStrictlySorted(l);
-  requires Keyspace.IsSorted(l);
-  requires pos == Keyspace.LargestLte(l, k);
+  requires Spec.CSMap.Keyspace.IsStrictlySorted(l);
+  requires Spec.CSMap.Keyspace.IsSorted(l);
+  requires pos == Spec.CSMap.Keyspace.LargestLte(l, k);
   requires pos < 0 || k != l[pos]
-  ensures Keyspace.IsStrictlySorted(insert(l,k,pos+1));
+  ensures Spec.CSMap.Keyspace.IsStrictlySorted(insert(l,k,pos+1));
   {
     var l' := insert(l,k,pos+1);
-    Keyspace.reveal_IsStrictlySorted();
+    Spec.CSMap.Keyspace.reveal_IsStrictlySorted();
 
     forall i, j | 0 <= i < j < |l'|
-    ensures Keyspace.lt(l'[i], l'[j])
+    ensures Spec.CSMap.Keyspace.lt(l'[i], l'[j])
     {
       reveal_insert();
     }
   }
 
   method empty<Value>()
-  returns (newtree: Node)
-  ensures WFRoot(newtree)
+  returns (newtree: Spec.Node)
+  ensures Spec.WFRoot(newtree)
   ensures CantEquivocate(newtree)
   {
-    Keyspace.reveal_IsStrictlySorted();
-    return Leaf([], [], Keyspace.Min_Element, Keyspace.Max_Element);
+    Spec.CSMap.Keyspace.reveal_IsStrictlySorted();
+    return Spec.Leaf([], [], Spec.CSMap.Keyspace.Min_Element, Spec.CSMap.Keyspace.Max_Element);
   }
 
-  method putInner<Value>(tree: Node, key: Key, value: Value)
-  returns (newtree: Node)
-  requires WFTree(tree)
-  requires Keyspace.lte(tree.lb, key);
-  requires Keyspace.lt(key, tree.ub);
-  ensures Put(Constants(), Variables(tree), Variables(newtree), key, value)
+  method putInner<Value>(tree: Spec.Node, key: Spec.Key, value: Value)
+  returns (newtree: Spec.Node)
+  requires Spec.WFTree(tree)
+  requires Spec.CSMap.Keyspace.lte(tree.lb, key);
+  requires Spec.CSMap.Keyspace.lt(key, tree.ub);
+  ensures Spec.Put(Spec.Constants(), Spec.Variables(tree), Spec.Variables(newtree), key, value)
   decreases tree
   {
     if (tree.Leaf?) {
-      Keyspace.IsStrictlySortedImpliesIsSorted(tree.keys);
-      var pos := Keyspace.LargestLte(tree.keys, key);
+      Spec.CSMap.Keyspace.IsStrictlySortedImpliesIsSorted(tree.keys);
+      var pos := Spec.CSMap.Keyspace.LargestLte(tree.keys, key);
       if (pos >= 0 && key == tree.keys[pos]) {
-        return Leaf(tree.keys, tree.values[pos := value], tree.lb, tree.ub);
+        return Spec.Leaf(tree.keys, tree.values[pos := value], tree.lb, tree.ub);
       } else {
         var newkeys := insert(tree.keys, key, pos+1);
         var newvals := insert(tree.values, value, pos+1);
         strictlySortedInsert(tree.keys, key, pos);
-        return Leaf(newkeys, newvals, tree.lb, tree.ub);
+        return Spec.Leaf(newkeys, newvals, tree.lb, tree.ub);
       }
     } else {
-      Keyspace.IsStrictlySortedImpliesIsSorted(tree.pivots);
-      var pos := Keyspace.LargestLte(tree.pivots, key) + 1;
+      Spec.CSMap.Keyspace.IsStrictlySortedImpliesIsSorted(tree.pivots);
+      var pos := Spec.CSMap.Keyspace.LargestLte(tree.pivots, key) + 1;
 
       if (pos == 0) {
         assert tree.children[pos].lb == tree.lb;
-        assert Keyspace.lte(tree.lb, key);
+        assert Spec.CSMap.Keyspace.lte(tree.lb, key);
       } else { 
         assert tree.children[pos].lb == tree.pivots[pos-1];
-        assert Keyspace.lte(tree.pivots[pos-1], key);
+        assert Spec.CSMap.Keyspace.lte(tree.pivots[pos-1], key);
       }
 
       var new_child := putInner(tree.children[pos], key, value);
       var new_children := tree.children[pos := new_child];
-      return Index(tree.pivots, new_children, tree.lb, tree.ub);
+      return Spec.Index(tree.pivots, new_children, tree.lb, tree.ub);
     }
   }
 
-  method put<Value>(tree: Node, key: Key, value: Value)
-  returns (newtree: Node)
-  requires WFRoot(tree)
-  requires Keyspace.lte(tree.lb, key);
-  requires Keyspace.lt(key, tree.ub);
-  ensures Put(Constants(), Variables(tree), Variables(newtree), key, value)
+  method put<Value>(tree: Spec.Node, key: Spec.Key, value: Value)
+  returns (newtree: Spec.Node)
+  requires Spec.WFRoot(tree)
+  requires Spec.CSMap.Keyspace.lte(tree.lb, key);
+  requires Spec.CSMap.Keyspace.lt(key, tree.ub);
+  ensures Spec.Put(Spec.Constants(), Spec.Variables(tree), Spec.Variables(newtree), key, value)
   decreases tree
   {
     if (tree.Leaf? && tree.keys == []) {
-      return Leaf([key], [value], tree.lb, tree.ub);
+      return Spec.Leaf([key], [value], tree.lb, tree.ub);
     } else {
       newtree := putInner(tree, key, value);
       return newtree;
